src/case_study/program_logic/gen_heap_lifting.v
@@ -1,0 +1,68 @@
+From iris.base_logic Require Export gen_heap.
+From iris.algebra Require Export list excl_auth.
+From iris.proofmode Require Import tactics.
+From stdpp Require Import fin_maps.
+From nextgen Require Import nextgen_basic nextgen_pointwise.
+Set Default Proof Using "Type".
+Import uPred.
+
+(** Some useful typeclasses for using IndInG/NoInG with gen_heaps and ghost_map *)
+
+Class ghost_mapIndG (Σ : gFunctors) (Ω : gTransformations Σ) (K V : Type) (eqdec: EqDecision K) (count: @Countable K eqdec) : Set := GhostMapIndG
+  { ghost_map_inIndG : genIndInG Σ Ω (gmap_view.gmap_viewR K (leibnizO V)) }.
+Arguments ghost_mapIndG Σ Ω (K V)%type_scope {_ _}.
+Arguments GhostMapIndG Σ Ω (K V)%type_scope {_ _ _}.
+
+Class ghost_mapNoG (Σ : gFunctors) (Ω : gTransformations Σ) (K V : Type)  (eqdec: EqDecision K) (count: @Countable K eqdec) : Set := GhostMapNoG
+  { ghost_map_inNoG : noTransInG Σ Ω (gmap_view.gmap_viewR K (leibnizO V)) }.
+Arguments ghost_mapNoG Σ Ω (K V)%type_scope {_ _}.
+Arguments GhostMapNoG Σ Ω (K V)%type_scope {_ _ _}.
+
+Class gen_heapNoGpreS (L V : Type) (Σ : gFunctors) (Ω : gTransformations Σ) (eqdec: EqDecision L) (count: Countable L) : Set := Build_gen_heapNoGpreS
+  { gen_heapNoGpreS_heap : ghost_mapNoG Σ Ω L V;
+    gen_heapNoGpreS_meta : ghost_mapIndG Σ Ω L gname;
+    gen_heapNoGpreS_meta_data : genIndInG Σ Ω (reservation_map.reservation_mapR (agreeR positiveO)) }.
+Arguments gen_heapNoGpreS (L V)%type_scope Σ Ω {_ _}.
+Arguments Build_gen_heapNoGpreS (L V)%type_scope Σ Ω {_ _ _ _ _}.
+
+Class gen_heapIndGpreS (L V : Type) (Σ : gFunctors) (Ω : gTransformations Σ) (eqdec: EqDecision L) (count: Countable L) : Set := Build_gen_heapIndGpreS
+  { gen_heapIndGpreS_heap : ghost_mapIndG Σ Ω L V;
+    gen_heapIndGpreS_meta : ghost_mapIndG Σ Ω L gname;
+    gen_heapIndGpreS_meta_data : genIndInG Σ Ω (reservation_map.reservation_mapR (agreeR positiveO)) }.
+Arguments gen_heapIndGpreS (L V)%type_scope Σ Ω {_ _}.
+Arguments Build_gen_heapIndGpreS (L V)%type_scope Σ Ω {_ _ _ _ _}.
+
+Class gen_heapNoGS (L V : Type) (Σ : gFunctors) (Ω : gTransformations Σ) (eqdec: EqDecision L) (count: Countable L) : Set := GenHeapNoGS
+  { gen_heap_inNoG : gen_heapNoGpreS L V Σ Ω;  no_gen_heap_name : gname;  no_gen_meta_name : gname }.
+Arguments gen_heapNoGS (L V)%type_scope Σ Ω {_ _}.
+Arguments GenHeapNoGS (L V)%type_scope Σ Ω {_ _ _} no_gen_heap_name no_gen_meta_name.
+
+Class gen_heapIndGS (L V : Type) (Σ : gFunctors) (Ω : gTransformations Σ) (eqdec: EqDecision L) (count: Countable L) : Set := GenHeapIndGS
+{ gen_heap_inIndG : gen_heapIndGpreS L V Σ Ω;  ind_gen_heap_name : gname;  ind_gen_meta_name : gname }.
+Arguments gen_heapIndGS (L V)%type_scope Σ Ω {_ _}.
+Arguments GenHeapIndGS (L V)%type_scope Σ Ω {_ _ _} ind_gen_heap_name ind_gen_meta_name.
+
+Class gen_heapNoMetaGS (L V : Type) (Σ : gFunctors) (Ω : gTransformations Σ) (eqdec: EqDecision L) (count: Countable L) : Set := GenHeapNoMetaGS
+  { gen_heap_inNoMetaG : ghost_mapNoG Σ Ω L V;  no_meta_gen_heap_name : gname; }.
+Arguments gen_heapNoMetaGS (L V)%type_scope Σ Ω {_ _}.
+Arguments GenHeapNoMetaGS (L V)%type_scope Σ Ω {_ _ _} no_meta_gen_heap_name.
+
+
+(** Some coersions from above classes to gen_heap/ghost_map *)
+
+#[global] Instance into_ghost_map_from_ind {K V Σ Ω} `{eqK: EqDecision K} `{countK: @Countable K eqK} (Hwsat: ghost_mapIndG Σ Ω K V) : ghost_map.ghost_mapG Σ K V :=
+  ghost_map.GhostMapG Σ K V eqK countK (Hwsat.(ghost_map_inIndG)).(genInG_inG).
+#[global] Instance into_ghost_map_from_no {K V Σ Ω} `{eqK: EqDecision K} `{countK: @Countable K eqK} (Hwsat: ghost_mapNoG Σ Ω K V) : ghost_map.ghost_mapG Σ K V :=
+  ghost_map.GhostMapG Σ K V eqK countK (Hwsat.(ghost_map_inNoG)).(noTransInG_inG).
+
+#[global] Instance into_gen_heap_pre_from_ind {L V Σ Ω} `{eqK: EqDecision L} `{countK: @Countable L eqK} (Hwsat: gen_heapIndGpreS L V Σ Ω) : gen_heapGpreS L V Σ :=
+  Build_gen_heapGpreS L V Σ eqK countK (into_ghost_map_from_ind gen_heapIndGpreS_heap) (into_ghost_map_from_ind gen_heapIndGpreS_meta) gen_heapIndGpreS_meta_data.(genInG_inG).
+
+#[global] Instance into_gen_heap_pre_from_no {L V Σ Ω} `{eqK: EqDecision L} `{countK: @Countable L eqK} (Hwsat: gen_heapNoGpreS L V Σ Ω) : gen_heapGpreS L V Σ :=
+  Build_gen_heapGpreS L V Σ eqK countK (into_ghost_map_from_no gen_heapNoGpreS_heap) (into_ghost_map_from_ind gen_heapNoGpreS_meta) gen_heapNoGpreS_meta_data.(genInG_inG).
+
+#[global] Instance into_gen_heap_from_ind {L V Σ Ω} `{eqK: EqDecision L} `{countK: @Countable L eqK} (Hwsat: gen_heapIndGS L V Σ Ω) : gen_heapGS L V Σ :=
+  @GenHeapGS L V Σ eqK countK (into_gen_heap_pre_from_ind gen_heap_inIndG) ind_gen_heap_name ind_gen_meta_name.
+
+#[global] Instance into_gen_heap_from_no {L V Σ Ω} `{eqK: EqDecision L} `{countK: @Countable L eqK} (Hwsat: gen_heapNoGS L V Σ Ω) : gen_heapGS L V Σ :=
+  @GenHeapGS L V Σ eqK countK (into_gen_heap_pre_from_no gen_heap_inNoG) no_gen_heap_name no_gen_meta_name.
